Graphiti/Core/Rewrites.lean
@@ -91,37 +91,37 @@ def rewrite_index :=
     ]
 
 def reverse_rewrite_with_index (rinfo : RuntimeEntry) : RewriteResult (Rewrite String (String × Nat)) := do
-  let rw ← ofOption (.error s!"{decl_name%}: rewrite generation failed") <| do
-    let name ← rinfo.name
+  let rw ← do
+    let name ← ofOption (.error s!"{decl_name%}: no rinfo report") rinfo.name
     match name with
     | "join-split-elim" =>
-      let s ← rinfo.matched_subgraph[0]?
+      let s ← ofOption (.error s!"{decl_name%}: 'join-split-elim' reverse rewrite generation failed") rinfo.matched_subgraph[0]?
       return JoinSplitElim.targetedRewrite s
     | "join-comm" =>
-      let s ← rinfo.matched_subgraph[0]?
+      let s ← ofOption (.error s!"{decl_name%}: 'join-comm' reverse rewrite generation failed") rinfo.matched_subgraph[0]?
       return JoinComm.targetedRewrite s
     | "join-assoc-right" =>
-      let s ← rinfo.matched_subgraph[0]?
+      let s ← ofOption (.error s!"{decl_name%}: 'join-assoc-right' reverse rewrite generation failed") rinfo.matched_subgraph[1]?
       return JoinAssocR.targetedRewrite s
     | "join-assoc-left" =>
-      let s ← rinfo.matched_subgraph[0]?
+      let s ← ofOption (.error s!"{decl_name%}: 'join-assoc-left' reverse rewrite generation failed") rinfo.matched_subgraph[1]?
       return JoinAssocL.targetedRewrite s
     | "pure-fork" =>
-      let s ← rinfo.matched_subgraph[0]?
+      let s ← ofOption (.error s!"{decl_name%}: 'pure-fork' reverse rewrite generation failed") rinfo.matched_subgraph[0]?
       return {PureRewrites.Fork.rewrite with pattern := PureRewrites.Fork.match_node s}
     | "pure-operator3" =>
-      let s ← rinfo.matched_subgraph[0]?
+      let s ← ofOption (.error s!"{decl_name%}: 'pure-operator3' reverse rewrite generation failed") rinfo.matched_subgraph[0]?
       return {PureRewrites.Operator3.rewrite with pattern := PureRewrites.Operator3.match_node s}
     | "pure-operator2" =>
-      let s ← rinfo.matched_subgraph[0]?
+      let s ← ofOption (.error s!"{decl_name%}: 'pure-operator2' reverse rewrite generation failed") rinfo.matched_subgraph[0]?
       return {PureRewrites.Operator2.rewrite with pattern := PureRewrites.Operator2.match_node s}
     | "pure-operator1" =>
-      let s ← rinfo.matched_subgraph[0]?
+      let s ← ofOption (.error s!"{decl_name%}: 'pure-operator1' reverse rewrite generation failed") rinfo.matched_subgraph[0]?
       return {PureRewrites.Operator1.rewrite with pattern := PureRewrites.Operator1.match_node s}
     | "pure-constant" =>
-      let s ← rinfo.matched_subgraph[0]?
+      let s ← ofOption (.error s!"{decl_name%}: 'constant' reverse rewrite generation failed") rinfo.matched_subgraph[0]?
       return {PureRewrites.Constant.rewrite with pattern := PureRewrites.Constant.match_node s}
-    | _ => rewrite_index.find? name
+    | s => ofOption (.error s!"{decl_name%}: '{s}' reverse rewrite generation failed") <| rewrite_index.find? name
   reverse_rewrite rw rinfo
 
 /--
