Graphiti/Core/Rewrites/JoinAssocR.lean
@@ -18,9 +18,9 @@ variable (M : Nat)
 
 def identMatcher (join2 : String) : Pattern String (String × Nat) 2 := fun g => do
   let join2_typ ← ofOption' (.error s!"{decl_name%}: could not find '{join2}'") <| g.modules.find? join2
-  unless "join" == join2_typ.2.1 do throw (.error s!"type of '{join2}' is '{join2_typ.2}' instead of 'join'")
+  unless "join" == join2_typ.2.1 do throw (.error s!"{decl_name%}: type of '{join2}' is '{join2_typ.2}' instead of 'join'")
   let join1 ← ofOption' (.error s!"{decl_name%}: could not find next node") <| followInput g join2 "in1"
-  unless "join" == join1.typ.1 do throw (.error s!"type of '{join1.inst}' is '{join1.typ}' instead of 'join'")
+  unless "join" == join1.typ.1 do throw (.error s!"{decl_name%}: type of '{join1.inst}' is '{join1.typ}' instead of 'join' 2")
 
   return ([join1.inst, join2], #v[join1.typ.2, join2_typ.2.2])
 
@@ -59,8 +59,8 @@ def rhs : ExprHigh String (String × Nat) := [graph|
     i_2 [type = "io"];
     o_out [type = "io"];
 
-    join2 [type = "split", arg = $(M+1)];
-    join1 [type = "split", arg = $(M+2)];
+    join2 [type = "join", arg = $(M+1)];
+    join1 [type = "join", arg = $(M+2)];
     pure [type = "pure", arg = $(M+3)];
 
     i_1 -> join2 [to = "in1"];
@@ -73,7 +73,7 @@ def rhs : ExprHigh String (String × Nat) := [graph|
     pure -> o_out [from = "out1"];
   ]
 
-def rhs_extract := (rhs M).extract ["join2", "join1", "pure"] |>.get rfl
+def rhs_extract := (rhs M).extract ["join1", "join2", "pure"] |>.get rfl
 def rhsLower := (rhs_extract M).fst.lower.get rfl
 def findRhs mod := (rhs_extract 0).fst.modules.find? mod |>.map Prod.fst
 
@@ -83,7 +83,7 @@ def rewrite : Rewrite String (String × Nat) :=
     pattern := matcher,
     rewrite := λ l n => ⟨lhsLower l, rhsLower n⟩
     name := "join-assoc-right"
-    transformedNodes := [findRhs "join2" |>.get rfl, findRhs "join1" |>.get rfl],
+    transformedNodes := [findRhs "join1" |>.get rfl, findRhs "join2" |>.get rfl],
     addedNodes := [findRhs "pure" |>.get rfl]
     fresh_types := 3
   }
